Fixed most things. One obdurate problem in FSExpGen o be fixed.

Src/BoogieExprTranslator/FlattenStmtLists.fs
@@ -1,0 +1,48 @@
+﻿namespace Microsoft.P2Boogie
+
+//Helper module to flatten all sequences of sequences. 
+//For aesthetic purposes, for now at least.
+module FlattenStmtLists = 
+  open Syntax
+  open Common
+
+  let rec flattenStmt st =
+    match st with
+    | Assign(_) | Insert(_)
+    | Remove(_)
+    | Assert(_)
+    | Assume(_)
+    | NewStmt(_)
+    | Raise(_)
+    | Send(_)
+    | Skip
+    | Pop
+    | Return(_)
+    | Monitor(_)
+    | FunStmt(_) -> [st]
+    | While(c, s) -> [While(c, (flattenAllStmts(flattenStmt s)))]
+    | Ite(c, i, e) -> 
+      [Ite(c, (flattenAllStmts(flattenStmt i)), (flattenAllStmts(flattenStmt e)))]
+    | SeqStmt(ls) -> 
+      List.fold (fun acc s -> acc @ (flattenStmt s)) [] ls
+    | Receive(ls) -> 
+        [Receive(List.map (fun (e, st) -> (e, flattenAllStmts(flattenStmt st))) ls)]
+      
+  and flattenAllStmts stlst = 
+    match stlst with
+    | [s] -> s
+    | h::t -> SeqStmt(stlst)
+    | _ -> raise NotDefined
+  
+  let flattenStmtsFun (fd: FunDecl) = 
+    let flatSt = List.fold (fun acc st -> acc @ (flattenStmt st)) [] fd.Body
+    new FunDecl(fd.Name, fd.Formals, fd.RetType, fd.Locals, flatSt, fd.IsModel, fd.IsPure)
+  
+  let flattenStmtsMachine (md: MachineDecl) = 
+    let fLst = List.map flattenStmtsFun md.Functions
+    new MachineDecl(md.Name, md.StartState, md.Globals, fLst, md.States, md.IsMonitor, md.MonitorList, md.QC, md.IsModel, md.HasPush)
+
+  let flattenStmtsProg (prog: ProgramDecl) = 
+    let fLst = List.map flattenStmtsFun prog.StaticFuns
+    let mLst = List.map flattenStmtsMachine prog.Machines
+    new ProgramDecl(prog.MainMachine, prog.Machines, prog.Events, prog.EventsToMonitors, prog.StaticFuns, prog.maxFields, prog.HasDefer, prog.HasIgnore)
